dafny/src/lendingProtocol.dfy
@@ -2,11 +2,13 @@
 include "util/number.dfy"
 include "util/maps.dfy"
 include "util/tx.dfy"
+include "fixed.dfy"
 
 
 import opened Number
 import opened Maps
 import opened Tx
+import opened Fixed
 
 
 class LendingProtocol {
@@ -22,17 +24,44 @@ class LendingProtocol {
     var usersCollateral: mapping<u160, u256>
     var usersBorrowed: mapping<u160, u256>
 
+    var WAD: u256
+
     constructor() {
         maxLTV := 4;
         baseRate := 20000000000000000;
         fixedAnnuBorrowRate := 300000000000000000;
 
+        WAD := 1000000000000000000;
+
         usersCollateral := Map(map[], 0);
         usersBorrowed := Map(map[], 0);
     }
 
-    method bondAsset(msg: Transaction) returns (r: Result<()>)
-    modifies this`totalDeposit {
+    method utilizationRatio() returns (utilizationRatio: u256)
+    ensures utilizationRatio == this.totalBorrow / this.totalDeposit
+    {
+        utilizationRatio := Fixed.Div(this.totalBorrow, this.totalDeposit);
+    }
+
+    method interestMultiplier() returns (interestMultiplier: u256)
+    {
+        var uRatio: u256 := utilizationRatio();
+        var num: u256 := Sub(this.fixedAnnuBorrowRate, this.baseRate);
+        interestMultiplier := Fixed.Div(num, uRatio);
+    }
+    
+
+    method borrowRate() returns (rate: u256)
+    requires rate > 0 {
+        var uRatio: u256 := utilizationRatio();
+
+    }
+
+
+    method calculateBorrowFee(amount: u256) returns (fee: u256, paid: u256)
+    requires amount > 0
+
+    {
         totalDeposit := totalDeposit;
         return Ok(());
     }
